Extraction of Dexter 2. WIP

extraction/theories/CameLIGOPretty.v
@@ -29,8 +29,67 @@ Notation "f <| x" := (f x) (at level 32, left associativity, only parsing).
 Notation "x |> f" := (f x) (at level 31, left associativity, only parsing).
 (* i.e. x |> f |> g = (x |> f) |> g, and means g (f x) *)
 
+Class CameLIGOPrintConfig :=
+  { (* cosnstructors start with an uppercase letter *)
+    print_ctor_name : kername -> string;
 
-Section print_term.
+    (* types start with a lowercase letter  *)
+    print_type_name : kername -> string;
+
+    (* constants start with a lowercase letter *)
+    print_const_name : kername -> string }.
+
+(** Prepend the last module name all global declaration names to avoid name clashes.  Due
+    to limitations for constructors, use only part of the module name and cut the first
+    31 letters *)
+Module PrintConfAddModuleNames.
+
+  Definition last_module_name (mp : modpath) : string :=
+    match mp with
+    | MPdot mp' nm => nm
+    | MPfile (nm :: _) => nm
+    | _ => ""
+    end.
+
+  Definition print_ctor_name_ (kn : kername) :=
+    let lmn := last_module_name kn.1 in
+    let nm := kn.2 in
+    (* NOTE: CameLIGO has a limitation for the constructor name length, so we try our best to fit and don't get clashes *)
+    let ctor_name := if lmn =? "" then nm else substring 0 4 lmn ^ "_" ^ nm in
+    capitalize (substring 0 31 ctor_name).
+
+  Definition print_ind_type_name_ (ind_kn : kername) :=
+    let lmn := last_module_name ind_kn.1 in
+    let nm := ind_kn.2 in
+    let ty_name := if lmn =? "" then nm else lmn ^ "_" ^ nm in
+    uncapitalize ty_name.
+
+  Definition print_const_name_ (ind_kn : kername) :=
+    let lmn := last_module_name ind_kn.1 in
+    let nm := ind_kn.2 in
+    let ty_name := if lmn =? "" then nm else lmn ^ "_" ^ nm in
+    uncapitalize ty_name.
+  
+  Local Instance PrintWithModuleNames : CameLIGOPrintConfig :=
+    {| print_ctor_name := print_ctor_name_;
+       print_type_name := print_ind_type_name_;
+       print_const_name := print_const_name_ |}.
+
+End PrintConfAddModuleNames.
+
+(** Print names only, don't prepend module names or any other parts of the fully qualified path.
+    Gives more readable code, but might lead to name clashes *)
+Module PrintConfShortNames.
+
+  Local Instance PrintWithShortNames : CameLIGOPrintConfig :=
+    {| print_ctor_name := fun kn => capitalize kn.2;
+       print_type_name := fun kn => uncapitalize kn.2;
+       print_const_name := fun kn => uncapitalize kn.2 |}.
+
+End PrintConfShortNames.
+
+Section PPTerm.
+  Context `{CameLIGOPrintConfig}.
   Context (Σ : ExAst.global_env).
 
   Definition look (e : MyEnv.env string) (s : string) : option string :=
@@ -66,13 +125,17 @@ Section print_term.
                     | _ => []
                     end.
 
+  
   Fixpoint get_tapp_hd (bt : box_type) : box_type :=
     match bt with
     | TApp t1 t2 => get_tapp_hd t1
     | _ => bt
     end.
 
-  Definition print_box_type (prefix : string) (TT : env string)
+  Definition print_type_var (i : nat) :=
+        "'a" ++ string_of_nat i.
+
+  Definition print_box_type (TT : env string)
     : box_type -> string :=
     fix go  (bt : box_type) :=
   match bt with
@@ -91,60 +154,61 @@ Section print_term.
       else print_uncurried "" args ++ " " ++ go hd
     | _ => print_uncurried "" args ++ " " ++ go hd
     end
-  | TVar i => "a" ++ string_of_nat i (* TODO: pass context with type variables *)
+  | TVar i => print_type_var i (* TODO: pass context with type variables *)
   | TInd s =>
     let full_ind_name := string_of_kername s.(inductive_mind) in
-    uncapitalize (from_option (look TT full_ind_name) (prefix ++ s.(inductive_mind).2))
+    from_option (look TT full_ind_name)
+                (print_type_name s.(inductive_mind))
   | TConst s =>
     let full_cst_name := string_of_kername s in
-    uncapitalize (from_option (look TT full_cst_name) (prefix ++ s.2))
-
+    from_option (look TT full_cst_name) (print_type_name s)
   | TAny => "UnknownType"
   end.
 
-  Definition print_ctor_name (prefix : string) (nm : string) :=
-    capitalize (prefix ^ nm).
-
   Definition print_ctor
-             (prefix : string)
              (TT : env string)
+             (ind_kn : kername)
              (ctor : ident × list (name × box_type)) :=
     let (nm,tys) := ctor in
-    (* cameligo constructors must start with a capital letter *)
-    let nm := print_ctor_name prefix nm in
+    let nm := print_ctor_name (ind_kn.1, nm) in
     match tys with
     | [] => nm
-    | _ => let ctor_type := parens false <| concat " * " (map (print_box_type prefix TT ∘ snd) tys)
+    | _ => let ctor_type := parens false <| concat " * " (map (print_box_type TT ∘ snd) tys)
           in nm ^ " of " ^ ctor_type
     end.
 
-  Definition print_proj (prefix : string) (TT : env string) (proj : ident × box_type) : string :=
+  Definition print_proj (TT : env string) (proj : ident × box_type) : string :=
     let (nm, ty) := proj in
-    let nm := prefix ^ nm in
-    nm ^ " : " ^ print_box_type prefix TT ty.
+    nm ^ " : " ^ print_box_type TT ty.
 
-  Definition print_inductive (prefix : string) (TT : env string)
+  Definition print_type_params (vs : list type_var_info) : string :=
+    if (Nat.eqb #|vs| 0) then ""
+      else (let ps := concat "," (mapi (fun i _ => print_type_var i) vs) in
+            (parens (Nat.eqb #|vs| 1) ps ^ " ")).
+
+  Definition print_type_declaration (nm : string) (params : list type_var_info) (body : string) : string :=
+    "type " ^ print_type_params params ^ nm ^ " = " ^ body.
+  
+  Definition print_inductive (ind_kn : kername) (TT : env string)
              (oib : ExAst.one_inductive_body) :=
     let ind_nm := from_option (lookup TT oib.(ExAst.ind_name))
-                              (prefix ++ oib.(ExAst.ind_name)) in
-    let print_type_var (i : nat) :=
-        "'a" ++ string_of_nat i in
-    let params :=
-      if (Nat.eqb #|oib.(ind_type_vars)| 0) then ""
-      else let ps := concat "," (mapi (fun i _ => print_type_var i) oib.(ind_type_vars)) in
-           (parens (Nat.eqb #|oib.(ind_type_vars)| 1) ps) ++ " " in
+                              (print_type_name (ind_kn.1, oib.(ExAst.ind_name))) in
     (* one-constructor inductives are interpreted/printed as records *)
     match oib.(ExAst.ind_ctors), oib.(ExAst.ind_projs) with
     | [build_record_ctor], _::_ =>
       let '(_, ctors) := build_record_ctor in
       let projs_and_ctors := combine oib.(ExAst.ind_projs) ctors in
-      let projs_and_ctors_printed := map (fun '(p, (na, ty)) => print_proj prefix TT (p.1, ty)) projs_and_ctors in
-      "type " ++ params ++ uncapitalize ind_nm ++ " = {" ++ nl
-              ++ concat (";" ++ nl) projs_and_ctors_printed ++ nl
-              ++  "}"
-    | _,_ => "type " ++ params ++ uncapitalize ind_nm ++ " = "
-                   ++ nl ++ "  "
-                   ++ concat "| " (map (fun p => print_ctor prefix TT p ++ nl) oib.(ExAst.ind_ctors))
+      let projs_and_ctors_printed := map (fun '(p, (na, ty)) => print_proj TT (p.1, ty)) projs_and_ctors in
+      let body :=
+        <$ "{";
+             concat (";" ^ nl) projs_and_ctors_printed;
+           "}" $> in
+      print_type_declaration ind_nm oib.(ind_type_vars) body
+    | _,_ =>
+        let body :=
+          <$ "";
+             "  " ^ concat "| " (map (fun p => print_ctor TT ind_kn p ^ nl) oib.(ExAst.ind_ctors)) $> in
+        print_type_declaration ind_nm oib.(ind_type_vars) body
     end.
 
   Definition is_sort (t : Ast.term) :=
@@ -363,12 +427,12 @@ Section print_term.
         ++ nl
         ++ print_term (ctx ++ ctx' ++ ctx)%list true false (lam_body fdef.(dbody)).
 
-  Definition print_pat (prefix : string) (TT : env string) (ctor : string) (infix : bool) (pt : list string * string) :=
+  Definition print_pat (TT : env string) (ind_kn : kername) (ctor : string) (infix : bool) (pt : list string * string) :=
     let vars := rev pt.1 in
     if infix then
       concat (" " ++ ctor ++ " ") vars ++ " -> " ++ pt.2
     else
-      let ctor_nm := from_option (look TT ctor) (print_ctor_name prefix ctor) in
+      let ctor_nm := from_option (look TT ctor) (print_ctor_name (ind_kn.1, ctor)) in
       let ctor_nm := if ctor_nm =? "Pair" then "" else ctor_nm in
       let print_parens := (Nat.ltb 1 (List.length pt.1)) in
       print_uncurried ctor_nm vars ++ " -> " ++ pt.2.
@@ -411,8 +475,7 @@ Section print_term.
 
   (** ** The pretty-printer *)
 
-  (** [prefix] - a sting pre-pended to the constants' and constructors' names to avoid clashes
-      [FT] - list of fixpoint names. Used to determine if uncurrying is needed for an applied variable (if it corresponds to a recursive call). The initial value is an empty list. Once we fit a fixpoint case, we add the fixpoint name to [FT], so all the recursive calls in the fixpoint body are packed into a tuple.
+  (** [FT] - list of fixpoint names. Used to determine if uncurrying is needed for an applied variable (if it corresponds to a recursive call). The initial value is an empty list. Once we fit a fixpoint case, we add the fixpoint name to [FT], so all the recursive calls in the fixpoint body are packed into a tuple.
 
       [TT] - translation table allowing for remapping constants and constructors to CameLIGO primitives, if required.
 
@@ -423,8 +486,7 @@ Section print_term.
       [t] - a term to be printed.
    *)
 
-  Fixpoint print_term (prefix : string)
-                      (FT : list string)
+  Fixpoint print_term (FT : list string)
                       (TT : env string)
                       (ctx : context)
                       (top : bool)
@@ -448,30 +510,31 @@ Section print_term.
       let na' := fresh_name ctx na t in
       let (dom_tys, _) := ExAst.decompose_arr bt in
       let dom_ty := match nth_error dom_tys 0 with
-                    | Some ty => print_box_type prefix TT ty
+                    | Some ty => print_box_type TT ty
                     | None => "LambdaError(NotAnArrowType)"
                     end in
       parens top ("fun (" ++ string_of_name ctx na' ++ " : "
                           ++ dom_ty ++ ")"
-                          ++ " -> " ++ print_term prefix FT TT (vass na' :: ctx) true false body a)
+                          ++ " -> " ++ print_term  FT TT (vass na' :: ctx) true false body a)
     | tLetIn na def body => fun '(bt, (vala, bodya)) =>
       let na' := fresh_name ctx na t in
       parens top ("let " ++ string_of_name ctx na' ++
-                        " = " ++ print_term prefix FT TT ctx true false def vala ++ " in " ++ nl ++
-                        print_term prefix FT TT (vdef na' def :: ctx) true false body bodya)
+                        " = " ++ print_term  FT TT ctx true false def vala ++ " in " ++ nl ++
+                        print_term  FT TT (vdef na' def :: ctx) true false body bodya)
     | tApp f l as t => fun '(bt, (fa, la)) =>
       let is_not_empty_const := fun t =>
         match t with
         | tApp t1 (tConst c as t2) =>
           let cst_name := string_of_kername c in
-          let nm := from_option (look TT cst_name) (prefix ++ c.2) in
+          let nm := from_option (look TT cst_name) c.2 in
           if nm =? "" then false
           else true
         | _ => true end in
-      let apps := rev (app_args_annot_empty_filtered (fun '(t; a) => print_term prefix FT TT ctx false false t a) (fun '(t';_) => is_not_empty_const t') t (bt, (fa, la))) in
+      (* FIXME: remove filtering of the arguments *)
+      let apps := rev (app_args_annot_empty_filtered (fun '(t; a) => print_term  FT TT ctx false false t a) (fun '(t';_) => is_not_empty_const t') t (bt, (fa, la))) in
       let '((b;ba),argas) := Edecompose_app_annot f fa in
       match apps with
-      | [] => print_term prefix FT TT ctx false true f fa
+      | [] => print_term  FT TT ctx false true f fa
       | _ =>
         match b with
           (* if the variable corresponds to a fixpoint, we pack the arguments into a tuple *)
@@ -481,27 +544,17 @@ Section print_term.
             let nm := (string_of_name ctx d.(decl_name)) in
             if List.in_dec String.string_dec nm FT
             then parens top (print_uncurried nm apps)
-            else parens (top || inapp) (print_term prefix FT TT ctx false true f fa ++ " " ++ print_term prefix FT TT ctx false false l la)
+            else parens (top || inapp) (print_term  FT TT ctx false true f fa ++ " " ++ print_term  FT TT ctx false false l la)
           | None => "UnboundRel(" ++ string_of_nat i ++ ")"
           end
         | tConst c =>
           let cst_name := string_of_kername c in
-          let nm := from_option (look TT cst_name) (prefix ++ c.2) in
+          let nm := from_option (look TT cst_name) (print_const_name c) in
           (* primitive projections instead of 'fst' and 'snd' *)
           if nm =? "fst" then
             (concat " " (map (parens true) apps)) ++ ".0"
           else if nm =? "snd" then
             (concat " " (map (parens true) apps)) ++ ".1"
-          (* Map Chain fields to record projections *)
-          else if (nm =? "chain_height") || (nm =? "current_slot") || (nm =? "finalized_height")  then
-            (concat " " (map (parens true) apps)) ++ "." ++ nm
-          (* ContractCallContext remappings *)
-          else if (nm =? "ctx_from") then
-            "Tezos.sender"
-          else if (nm =? "ctx_contract_address") then
-            "Tezos.self_address"
-          else if (nm =? "ctx_amount") then
-            "Tezos.amount"
           else parens (top || inapp) (nm ++ " " ++ (concat " " (map (parens true) apps)))
         | tConstruct (mkInd mind j as ind) i =>
           let nm := get_constr_name ind i in
@@ -526,24 +579,24 @@ Section print_term.
                   let projs_and_apps := combine (map fst oib.(ExAst.ind_projs)) apps in 
                   let field_decls_printed := projs_and_apps |> map (fun '(proj, e) => proj ++ " = " ++ e)
                                                           |> concat "; " in
-                  "({" ++ field_decls_printed ++ "}: " ++ print_box_type prefix TT bt ++ ")"
+                  "({" ++ field_decls_printed ++ "}: " ++ print_box_type  TT bt ++ ")"
                 | _,_ => 
                   (* constructors must be capitalized *)
-                  let nm' := from_option (look TT nm) (print_ctor_name prefix nm) in
+                  let nm' := from_option (look TT nm) (print_ctor_name (mind.1, nm)) in
                   parens top (print_uncurried nm' apps)
                 end
               end
         | _ => if is_not_empty_const l then
-                parens (top || inapp) (print_term prefix FT TT ctx false true f fa ++ " " ++ print_term prefix FT TT ctx false false l la)
-               else print_term prefix FT TT ctx false true f fa
+                parens (top || inapp) (print_term  FT TT ctx false true f fa ++ " " ++ print_term  FT TT ctx false false l la)
+               else print_term  FT TT ctx false true f fa
         end
       end
     | tConst c => fun bt =>
       let cst_name := string_of_kername c in
-      let nm_tt := from_option (look TT cst_name) (prefix ++ c.2) in
+      let nm_tt := from_option (look TT cst_name) (print_const_name c) in
       (* empty maps require type annotations *)
       if (nm_tt =? "Map.empty") || (nm_tt =? "AddressMap.empty") then
-        "(Map.empty: " ++ print_box_type prefix TT bt ++ ")"
+        "(Map.empty: " ++ print_box_type  TT bt ++ ")"
       else
         nm_tt
     | tConstruct ind l => fun bt =>
@@ -551,12 +604,12 @@ Section print_term.
       match print_num_literal TT t with
       | Some lit => lit
       | None =>
-        let nm_tt := from_option (look TT nm) (print_ctor_name prefix nm) in
+        let nm_tt := from_option (look TT nm) (print_ctor_name (ind.(inductive_mind).1, nm)) in
      (* NOTE: print annotations for 0-ary constructors of polymorphic types (like [], None, and Map.empty) *)
         if (uncapitalize nm =? "nil") && (eq_kername ind.(inductive_mind) <%% list %%>) then
-        "([]:" ++ print_box_type prefix TT bt ++ ")"
+        "([]:" ++ print_box_type  TT bt ++ ")"
         else if (nm =? "None") && (eq_kername ind.(inductive_mind) <%% option %%>) then
-               "(" ++ nm_tt ++ ":" ++ print_box_type prefix TT bt ++ ")"
+               "(" ++ nm_tt ++ ":" ++ print_box_type  TT bt ++ ")"
              else nm_tt
       end
     | tCase (mkInd mind i as ind, nparam) t brs =>
@@ -571,20 +624,20 @@ Section print_term.
               (* Assuming all case-branches have been expanded this should never happen: *)
               | t => fun btt => (params , "ERROR: unexpected wildcard branch - currently not supported")
             end
-            | 0 => fun bt => (params , print_term prefix FT TT ctx false false br bt)
+            | 0 => fun bt => (params , print_term FT TT ctx false false br bt)
             end in
 
       match brs with
-      | [] => fun '(bt, (ta, trs)) => (parens false ("failwith 0 : " ^ print_box_type prefix TT bt) ^ " (* absurd case *)")
+      | [] => fun '(bt, (ta, trs)) => (parens false ("failwith 0 : " ^ print_box_type  TT bt) ^ " (* absurd case *)")
       | _ =>
         (* [if-then-else] is a special case *)
         if eq_kername mind <%% bool %%> then
           match brs with
           | [b1;b2] => fun '(bt, (ta, (b1a, (b2a, _)))) =>
             parens top
-                    ("if " ++ print_term prefix FT TT ctx true false t ta
-                           ++ " then " ++ print_term prefix FT TT ctx true false (snd b1) b1a
-                           ++ " else " ++ print_term prefix FT TT ctx true false (snd b2) b2a)
+                    ("if " ++ print_term  FT TT ctx true false t ta
+                           ++ " then " ++ print_term  FT TT ctx true false (snd b1) b1a
+                           ++ " else " ++ print_term  FT TT ctx true false (snd b2) b2a)
           | _ => fun bt => "Error (Malformed pattern-mathing on bool: given "
                    ++ string_of_nat (List.length brs) ++ " branches " ++ ")"
           end
@@ -601,14 +654,14 @@ Section print_term.
               print_list (fun '(b, (na, _)) =>
                             (* [list] is a special case *)
                             if (eq_kername mind <%% list %%>) && (na =? "cons") then
-                              print_pat prefix TT "::" true b
-                            else if (eq_kername mind <%% list %%>) && (na =? "nil") then
-                              print_pat "" TT "[]" false b
+                              print_pat  TT mind "::" true b
+                            (* else if (eq_kername mind <%% list %%>) && (na =? "nil") then *)
+                            (*   print_pat "" TT mind "[]" false b *)
                             else
-                            print_pat prefix TT na false b)
+                            print_pat TT mind na false b)
                          (nl ++ " | ") brs_ in
            parens top
-                  ("match " ++ print_term prefix FT TT ctx true false t ta
+                  ("match " ++ print_term  FT TT ctx true false t ta
                             ++ " with " ++ nl
                             ++ brs_printed)
         | None =>
@@ -620,19 +673,19 @@ Section print_term.
       match lookup_ind_decl mind i with
       | Some oib =>
         match nth_error oib.(ExAst.ind_projs) k with
-        | Some (na, _) => print_term prefix FT TT ctx false false c bt.2 ++ "." ++ na
+        | Some (na, _) => print_term  FT TT ctx false false c bt.2 ++ "." ++ na
         | None => "UnboundProj(" ++ string_of_inductive ind ++ "," ++ string_of_nat i ++ "," ++ string_of_nat k ++ ","
-                  ++ print_term prefix FT TT ctx true false c bt.2 ++ ")"
+                  ++ print_term  FT TT ctx true false c bt.2 ++ ")"
         end
       | None =>
         "UnboundProj(" ++ string_of_inductive ind ++ "," ++ string_of_nat i ++ "," ++ string_of_nat k ++ ","
-                       ++ print_term prefix FT TT ctx true false c bt.2 ++ ")"
+                       ++ print_term  FT TT ctx true false c bt.2 ++ ")"
       end
     | tFix [fix_decl] n => fun '(bt, (fixa, _)) => (* NOTE: We assume that the fixpoints are not mutual *)
         (* Given an arrow type, prints the arguments in a curried way *)
-        let print_args_curried prefix TT ctx bt args :=
+        let print_args_curried  TT ctx bt args :=
           let (tys,_) := decompose_arr bt  in
-          let targs := combine args (map (print_box_type prefix TT) tys) in
+          let targs := combine args (map (print_box_type  TT) tys) in
           targs
             |> map (fun '(x,ty) => parens false (string_of_name ctx x ++ " : " ++ ty) )
             |> concat " " in
@@ -641,7 +694,7 @@ Section print_term.
         let '(args, (lam_body; body_annot)) := Edecompose_lam_annot body fixa in
 
         let sargs := map (string_of_name ctx) args in
-        let sargs_typed := print_args_curried prefix TT ctx bt args in
+        let sargs_typed := print_args_curried  TT ctx bt args in
         let fix_call :=
             "fun " ++ sargs_typed ++ " -> "
                    ++ print_uncurried fix_name sargs in
@@ -655,13 +708,13 @@ Section print_term.
           let '(args,(lam_body; body_annot)) := Edecompose_lam_annot (fdef.(dbody)) btt in
           let ctx := rev (map vass args) in
           let sargs := map (string_of_name ctx) args in
-          let tys_printed := map (print_box_type prefix TT) tys in
+          let tys_printed := map (print_box_type  TT) tys in
           let sargs_uncurried := parens false (concat ", " sargs ++ " : " ++ concat " * " tys_printed) in
-          let ret_ty_printed := print_box_type prefix TT ret_ty in
+          let ret_ty_printed := print_box_type  TT ret_ty in
               string_of_name ctx fdef.(dname) ++ " " ++ sargs_uncurried  ++
               " : " ++ ret_ty_printed ++ " = "
               ++ nl
-              ++ lam_body_annot_cont (fun body body_annot => print_term prefix FT' TT (ctx ++ ctx' ++ ctx)%list true false body body_annot) fdef.(dbody) btt
+              ++ lam_body_annot_cont (fun body body_annot => print_term  FT' TT (ctx ++ ctx' ++ ctx)%list true false body body_annot) fdef.(dbody) btt
         in
         parens top ("let rec " ++ print_def_annot ctx fix_decl fixa ++ nl ++
                                " in " ++ fix_call)
@@ -671,334 +724,341 @@ Section print_term.
     | tPrim _ => fun _ => "NotSupportedCoqPrimitive"
   end.
 
-End print_term.
+End PPTerm.
 
-Fixpoint get_fix_names (t : term) : list name :=
-  match t with
-  | tEvar _ args => List.concat (map get_fix_names args)
-  | tLambda _ b => get_fix_names b
-  | tLetIn _ t1 t2 => get_fix_names t1 ++ get_fix_names t2
-  | tApp t1 t2 => get_fix_names t1 ++ get_fix_names t2
-  | tCase _ t1 brs => get_fix_names t1
-                        ++ List.concat (map (get_fix_names ∘ snd) brs)
-  | tProj _ t1 => get_fix_names t1
-  | tFix mfix _ => map dname mfix ++ List.concat (map (get_fix_names ∘ dbody) mfix)
-  | tCoFix mfix _ => map dname mfix ++ List.concat (map (get_fix_names ∘ dbody) mfix)
-  | _ => []
-  end.
+Section PPLigo.
 
-Definition print_decl (prefix : string)
-           (TT : MyEnv.env string) (* translation table *)
-           (env : ExAst.global_env)
-           (decl_name : string)
-           (modifier : option string)
-           (wrap : string -> string)
-           (ty : box_type)
-           (t : term)
-           (ta : annots box_type t)
-            :=
-  let (tys,_) := decompose_arr ty in
-  let '(args,(lam_body; body_annot)) := Edecompose_lam_annot t ta in
-  let (ctx, args) := fresh_names [] args in
-  let targs := combine args (map (print_box_type prefix TT) tys) in
-  let printed_targs :=
-      map (fun '(x,ty) => parens false (string_of_name ctx x ++ " : " ++ ty)) targs in
-  let decl := prefix ++ decl_name ++ " " ++ concat " " printed_targs in
-    "let" ++ " " ++ decl ++ " = "
-          ++ wrap (CameLIGOPretty.print_term env prefix [] TT ctx true false lam_body body_annot).
+  Context `{CameLIGOPrintConfig}.
 
-Definition print_init (prefix : string)
-           (TT : MyEnv.env string) (* translation table *)
-           (build_call_ctx : string) (* a string that corresponds to a call contex *)
-           (init_prelude : string) (* operations available in the [init] as local definitions.
-                                      CameLIGO does not allow to refer to global definitions in [init]*)
-           (env : ExAst.global_env)
-           (cst : ExAst.constant_body)
-           : (constant_body_annots box_type cst) -> option string :=
+  Definition print_decl
+             (TT : MyEnv.env string) (* translation table *)
+             (env : ExAst.global_env)
+             (decl_kn : kername)
+             (wrap : string -> string)
+             (ty : box_type)
+             (t : term)
+             (ta : annots box_type t)
+    :=
+    let (tys,_) := decompose_arr ty in
+    let '(args,(lam_body; body_annot)) := Edecompose_lam_annot t ta in
+    let (ctx, args) := fresh_names [] args in
+    let targs := combine args (map (print_box_type TT) tys) in
+    let printed_targs :=
+        map (fun '(x,ty) => parens false (string_of_name ctx x ++ " : " ++ ty)) targs in
+    let decl := print_const_name decl_kn ++ concat " " printed_targs in
+      "let" ++ " " ++ decl ++ " = "
+            ++ wrap (print_term env [] TT ctx true false lam_body body_annot).
+
+  Definition print_init
+             (TT : MyEnv.env string) (* translation table *)
+             (build_call_ctx : string) (* a string that corresponds to a call contex *)
+             (init_prelude : string) (* operations available in the [init] as local definitions.
+                                        CameLIGO does not allow to refer to global definitions in [init]*)
+             (env : ExAst.global_env)
+             (cst : ExAst.constant_body)
+             : (constant_body_annots box_type cst) -> option string :=
+      match cst.(ExAst.cst_body) as body return match body with
+                                                | Some body => annots box_type body
+                                                | None => unit
+                                                end -> option string with
+      | Some b => fun cstAnnot =>
+      let '(args,(lam_body; body_annot)) := Edecompose_lam_annot b cstAnnot in
+      let ty := cst.(ExAst.cst_type) in
+      let (tys,inner_ret_ty) := decompose_arr ty.2 in
+      let targs_inner := combine args (map (print_box_type TT) tys) in
+      let ctx := map (fun x => Build_context_decl x None) (rev args) in
+      let printed_targs_inner :=
+          map (fun '(x,ty) => parens false (string_of_name ctx x ++ " : " ++ ty)) targs_inner in
+      let decl_inner := "inner " ++ concat " " printed_targs_inner in
+      let printed_inner_ret_ty := print_box_type TT inner_ret_ty in
+      let printed_outer_ret_ty :=
+        match inner_ret_ty with
+        | TApp (TInd ind) t1 =>
+          if eq_kername <%% option %%> ind.(inductive_mind) then
+            print_box_type TT t1
+          else print_box_type TT inner_ret_ty
+        | _ => print_box_type TT inner_ret_ty
+        end in
+      let wrap t :=
+        "match " ++ t ++ " with" ++ nl ++
+        "  Some v -> v"++ nl ++
+        "| None -> (failwith (""""): " ++ printed_outer_ret_ty ++ ")" in
+      let let_inner :=
+          "let " ++ decl_inner ++ " :" ++ printed_inner_ret_ty ++ " = " ++ nl
+                ++ print_term env [] TT ctx true false lam_body body_annot
+                ++ " in" in
+      (* if init takes no parameters, we give it a unit parameter  *)
+      let printed_targs_outer := match printed_targs_inner with
+                                 | _::[] | [] => let arg_name := fresh_name ctx nAnon tBox in
+                                         [parens false (string_of_name ctx arg_name ++ " : unit")]
+                                 | _::xs => xs
+                                 end in
+      (* ignore the first argument because it's a call context *)
+      let decl_outer :=
+        "init " ++ concat " " printed_targs_outer ++ " : " ++ printed_outer_ret_ty in
+      let let_ctx := "let ctx = " ++ build_call_ctx ++ " in" in
+      let inner_app := "inner " ++ concat " " ( "ctx" :: map (string_of_name ctx) (tl args)) in
+      let init_args_ty := "type init_args_ty = " ++
+        match tys with
+        | _::[] => "unit"
+        | [] => "unit"
+        | _::_ => tl tys |> map (print_box_type TT)
+                         |> concat " * "
+      end in
+      let init_wrapper_args_printed tys :=
+        match tys with
+        | [] => "()"
+        | [ty] => " args"
+        | tys => tys |> fold_right (fun _ '(i,s) => (i+1,s ++ " args." ++ string_of_nat i)) (0, "")
+                     |> snd
+        end in
+      let init_wrapper :=
+           "let init_wrapper (args : init_args_ty) ="
+        ++ nl
+        ++ "  init" ++ (tl tys |> init_wrapper_args_printed) in
+      ret ("let " ++ decl_outer ++ " = "
+                      ++ nl
+                      ++ init_prelude
+                      ++ nl
+                      ++ let_inner
+                      ++ nl
+                      ++ let_ctx
+                      ++ nl
+                      ++ wrap (parens false inner_app)
+                      ++ nl
+                      ++ init_args_ty
+                      ++ nl
+                      ++ init_wrapper
+                      ++ nl)
+    | None => fun _ => None
+    end.
+
+  Definition print_cst
+             (TT : MyEnv.env string) (* translation table *)
+             (env : ExAst.global_env)
+             (kn : kername)
+             (cst : ExAst.constant_body)
+             : (constant_body_annots box_type cst) -> option string :=
     match cst.(ExAst.cst_body) as body return match body with
                                               | Some body => annots box_type body
                                               | None => unit
                                               end -> option string with
-    | Some b => fun cstAnnot =>
-    let '(args,(lam_body; body_annot)) := Edecompose_lam_annot b cstAnnot in
-    let ty := cst.(ExAst.cst_type) in
-    let (tys,inner_ret_ty) := decompose_arr ty.2 in
-    let targs_inner := combine args (map (print_box_type prefix TT) tys) in
-    let ctx := map (fun x => Build_context_decl x None) (rev args) in
-    let printed_targs_inner :=
-        map (fun '(x,ty) => parens false (string_of_name ctx x ++ " : " ++ ty)) targs_inner in
-    let decl_inner := "inner " ++ concat " " printed_targs_inner in
-    let printed_inner_ret_ty := print_box_type prefix TT inner_ret_ty in
-    let printed_outer_ret_ty :=
-      match inner_ret_ty with
-      | TApp (TInd ind) t1 =>
-        if eq_kername <%% option %%> ind.(inductive_mind) then
-          print_box_type prefix TT t1
-        else print_box_type prefix TT inner_ret_ty
-      | _ => print_box_type prefix TT inner_ret_ty
-      end in
-    let wrap t :=
-      "match " ++ t ++ " with" ++ nl ++
-      "  Some v -> v" ++ nl ++
-      "| None -> (failwith (""""): " ++ printed_outer_ret_ty ++ ")" in
-    let let_inner :=
-        "let " ++ decl_inner ++ " :" ++ printed_inner_ret_ty ++ " = " ++ nl
-              ++ CameLIGOPretty.print_term env prefix [] TT ctx true false lam_body body_annot
-              ++ " in" in
-    (* if init takes no parameters, we give it a unit parameter  *)
-    let printed_targs_outer := match printed_targs_inner with
-                               | _::[] | [] => let arg_name := fresh_name ctx nAnon tBox in
-                                       [parens false (string_of_name ctx arg_name ++ " : unit")]
-                               | _::xs => xs
-                               end in
-    (* ignore the first argument because it's a call context *)
-    let decl_outer :=
-      "init " ++ concat " " printed_targs_outer ++ " : " ++ printed_outer_ret_ty in
-    let let_ctx := "let ctx = " ++ build_call_ctx ++ " in" in
-    let inner_app := "inner " ++ concat " " ( "ctx" :: map (string_of_name ctx) (tl args)) in
-    let init_args_ty := "type init_args_ty = " ++
-      match tys with
-      | _::[] => "unit"
-      | [] => "unit"
-      | _::_ => tl tys |> map (print_box_type prefix TT)
-                       |> concat " * "
-    end in
-    let init_wrapper_args_printed tys :=
-      match tys with
-      | [] => "()"
-      | [ty] => " args"
-      | tys => tys |> fold_right (fun _ '(i,s) => (i+1,s ++ " args." ++ string_of_nat i)) (0, "")
-                   |> snd
-      end in
-    let init_wrapper :=
-         "let init_wrapper (args : init_args_ty) ="
-      ++ nl
-      ++ "  init" ++ (tl tys |> init_wrapper_args_printed) in
-    ret ("let " ++ decl_outer ++ " = "
-                    ++ nl
-                    ++ init_prelude
-                    ++ nl
-                    ++ let_inner
-                    ++ nl
-                    ++ let_ctx
-                    ++ nl
-                    ++ wrap (parens false inner_app)
-                    ++ nl
-                    ++ init_args_ty
-                    ++ nl
-                    ++ init_wrapper
-                    ++ nl)
-  | None => fun _ => None
+    | Some cst_body => fun annot =>
+      (* NOTE: ignoring the path part *)
+      Some <| print_decl TT env kn id cst.(ExAst.cst_type).2 cst_body annot
+    | None => fun _ => None
+    end.
+
+  (* A wrapper type to separate declarations into type declarations ("type ... = ...")
+     and constant declarations ("let x = ...") *)
+  Inductive Decl a : Type :=
+    | TyDecl : a -> Decl a
+    | ConstDecl : a -> Decl a.
+  Global Arguments TyDecl {_}.
+  Global Arguments ConstDecl {_}.
+
+  Definition print_global_decl (TT : MyEnv.env string)
+             (nm : kername)
+             (env : ExAst.global_env)
+             (d : ExAst.global_decl) :
+             (global_decl_annots box_type d) -> Decl (kername * string) :=
+    match d return (global_decl_annots box_type d) -> Decl (kername * string) with
+    | ExAst.ConstantDecl cst => fun annot =>
+      match print_cst TT env nm cst annot with
+      | Some r => ConstDecl (nm, r)
+      | None =>  ConstDecl (nm, "print_global_decl ConstantDecl ERROR: " ++ string_of_kername nm)
+      end
+    | ExAst.InductiveDecl mib as d => fun annot =>
+      match mib.(ExAst.ind_bodies) with
+      | [oib] => TyDecl (nm, print_inductive nm TT oib)
+      | _ => TyDecl (nm,"Only non-mutual inductives are supported; " ++ string_of_kername nm)
+      end
+    | TypeAliasDecl (Some (params, ty)) => fun annot =>
+      let ta_nm := from_option (lookup TT (string_of_kername nm)) (print_type_name nm) in
+      TyDecl (nm, print_type_declaration ta_nm params (print_box_type TT ty))
+    | TypeAliasDecl None => fun _ => TyDecl (nm, "")
   end.
 
-Definition print_cst (prefix : string)
-           (TT : MyEnv.env string) (* translation table *)
-           (env : ExAst.global_env)
-           (kn : kername)
-           (cst : ExAst.constant_body)
-           : (constant_body_annots box_type cst) -> option string :=
-  match cst.(ExAst.cst_body) as body return match body with
-                                            | Some body => annots box_type body
-                                            | None => unit
-                                            end -> option string with
-  | Some cst_body => fun annot =>
-    (* NOTE: ignoring the path part *)
-    let (_, decl_name) := kn in
-    Some <| print_decl prefix TT env decl_name None id cst.(ExAst.cst_type).2 cst_body annot
-  | None => fun _ => None
-  end.
+  Fixpoint print_global_env (TT : MyEnv.env string)
+             (env : ExAst.global_env)
+             : (env_annots box_type env) -> list (Decl (kername * string)) :=
+    match env return (env_annots box_type env) -> list (Decl (kername * string)) with
+    | (kn, has_deps, decl) :: env' =>
+      fun '(a,b) =>
+        (* Filtering out empty type declarations *)
+        (* TODO: possibly, move to extraction (requires modifications of the correctness proof) *)
+        if is_empty_type_decl decl then print_global_env TT env' b
+        else
+          let printed :=
+          (* only print decls for which the environment includes dependencies *)
+          if has_deps then
+            print_global_decl TT kn env' decl a
+          else ConstDecl (kn, "") in
+      printed :: print_global_env TT env' b
+    | [] => fun _ => []
+    end.
 
-(* Wrapper type to separate declarations into type declarations ("type ... = ...")
-   and constant declarations ("let x = ...") *)
-Inductive Decl a : Type :=
-  | TyDecl : a -> Decl a
-  | ConstDecl : a -> Decl a.
-Arguments TyDecl {_}.
-Arguments ConstDecl {_}.
+  Local Open Scope string_scope.
 
-Definition print_global_decl (prefix : string) (TT : MyEnv.env string)
-           (nm : kername)
-           (env : ExAst.global_env)
-           (d : ExAst.global_decl) :
-           (global_decl_annots box_type d) -> Decl (kername * string) :=
-  match d return (global_decl_annots box_type d) -> Decl (kername * string) with
-  | ExAst.ConstantDecl cst => fun annot =>
-    match print_cst prefix TT env nm cst annot with
-    | Some r => ConstDecl (nm, r)
-    | None =>  ConstDecl (nm, "print_global_decl ConstantDecl ERROR?")
-    end
-  | ExAst.InductiveDecl mib as d => fun annot =>
-    match mib.(ExAst.ind_bodies) with
-    | [oib] => TyDecl (nm, print_inductive prefix TT oib)
-    | _ => TyDecl (nm,"Only non-mutual inductives are supported; " ++ string_of_kername nm)
-    end
-  | TypeAliasDecl (Some (params, ty)) => fun annot =>
-    let ta_nm := from_option (lookup TT (string_of_kername nm))
-                             (prefix ++ nm.2) in
-    TyDecl (nm, "type " ++ uncapitalize ta_nm ++ concat " " (map ((string_of_name []) ∘ tvar_name) params) ++  " = "
-            ++ print_box_type prefix TT ty)
-  | TypeAliasDecl None => fun _ => TyDecl (nm, "")
-end.
+  (** We un-overload operations and add definitions that are more convenient to use during the pretty-printing phase. These part should be included when printing contracts that use the corresponding operations. *)
 
-Fixpoint print_global_env (prefix : string) (TT : MyEnv.env string)
-           (env : ExAst.global_env)
-           : (env_annots box_type env) -> list (Decl (kername * string)) :=
-  match env return (env_annots box_type env) -> list (Decl (kername * string)) with
-  | (kn, has_deps, decl) :: env' =>
-    fun '(a,b) =>
-      (* Filtering out empty type declarations *)
-      (* TODO: possibly, move to extraction (requires modifications of the correctness proof) *)
-      if is_empty_type_decl decl then print_global_env prefix TT env' b
-      else
-        let printed :=
-        (* only print decls for which the environment includes dependencies *)
-        if has_deps then
-          print_global_decl prefix TT kn env' decl a
-        else ConstDecl (kn, "") in
-    printed :: print_global_env prefix TT env' b
-  | [] => fun _ => []
-  end.
+  Definition int_ops :=
+    <$
+    "[@inline] let addInt (i : int) (j : int) = i + j" ;
+    "[@inline] let subInt (i : int) (j : int) = i - j" ;
+    "[@inline] let subIntTruncated (a : int) (b : int) = let res = a - b in if res < 0 then 0 else res" ;
+    "[@inline] let multInt (i : int) (j : int) = i * j" ;
+    "[@inline] let divInt (i : int) (j : int) = i / j" ;
+    "[@inline] let modInt (a : int)(b : int) : int = int (a mod b)" ;
+    "[@inline] let leInt (i : int) (j : int) = i <= j" ;
+    "[@inline] let ltInt (i : int) (j : int) = i < j" ;
+    "[@inline] let eqInt (i : int) (j : int) = i = j"
+    $>.
 
+  Definition tez_ops :=
+    <$
+    "[@inline] let addTez (n : tez) (m : tez) = n + m" ;
+    "[@inline] let subTez (n : tez) (m : tez) = n - m" ;
+    "[@inline] let leTez (a : tez ) (b : tez ) = a <= b" ;
+    "[@inline] let ltTez (a : tez ) (b : tez ) =  a < b" ;
+    "[@inline] let gtbTez (a : tez ) (b : tez ) =  a > b" ;
+    "[@inline] let eqTez (a : tez ) (b : tez ) = a = b" ;
+    "[@inline] let natural_to_mutez (a: nat): tez = a * 1mutez" ;
+    "[@inline] let divTez (a : tez) (b : tez) : tez = natural_to_mutez (a/b)" ;
+    "[@inline] let multTez (n : tez) (m : tez) = (n/1tez) * m";
+    "[@inline] let evenTez (i : tez) = (i mod 2n) = 0tez"
+    $>.
+  Definition nat_ops :=
+    <$
+    "[@inline] let addN (a : nat ) (b : nat ) = a + b" ;
+    "[@inline] let multN (a : nat ) (b : nat ) = a * b" ;
+    "[@inline] let modN (a : nat ) (b : nat ) = a mod b" ;
+    "[@inline] let divN (a : nat ) (b : nat ) = a / b" ;
+    "[@inline] let eqN (a : nat ) (b : nat ) = a = b" ;
+    "[@inline] let lebN (a : nat ) (b : nat ) = a <= b" ;
+    "[@inline] let ltbN (a : nat ) (b : nat ) = a < b";
+    "let divN_opt (n : nat) (m : nat) : nat option = match ediv n m with | Some (q,_) -> Some q | None -> None";
+    "let moduloN (n : nat) (m : nat) : nat = match ediv n m with | Some (_,r) -> r | None -> 0n";
+    "let subOption (n : nat) (m : nat) : nat option = if n < m then None else Some (abs (n-m))";
+    "let z_to_N (i : int) : nat = if i < 0 then 0n else abs i";
+    "let z_of_N (n : nat) : int = int (n)"
+    $>.
 
-Local Open Scope string_scope.
+  Definition bool_ops :=
+    <$
+    "[@inline] let andb (a : bool ) (b : bool ) = a && b" ;
+    "[@inline] let orb (a : bool ) (b : bool ) = a || b"
+    $>.
 
-(** We un-overload operations and add definitions that are more convenient to use during the pretty-printing phase. These part should be included when printing contracts that use the corresponding operations. *)
+  Definition time_ops :=
+    <$
+    "[@inline] let eqb_time (a1 : timestamp) (a2 : timestamp) = a1 = a2" ;
+    "[@inline] let leb_time (a1 : timestamp) (a2 : timestamp) = a1 <= a2" ;
+    "[@inline] let ltb_time (a1 : timestamp) (a2 : timestamp) = a1 < a2"
+    $>.
 
-Definition int_ops :=
-  <$
-  "[@inline] let addInt (i : int) (j : int) = i + j" ;
-  "[@inline] let subInt (i : int) (j : int) = i - j" ;
-  "[@inline] let subIntTruncated (a : int) (b : int) = let res = a - b in if res < 0 then 0 else res" ;
-  "[@inline] let multInt (i : int) (j : int) = i * j" ;
-  "[@inline] let divInt (i : int) (j : int) = i / j" ;
-  "[@inline] let modInt (a : int)(b : int) : int = int (a mod b)" ;
-  "[@inline] let leInt (i : int) (j : int) = i <= j" ;
-  "[@inline] let ltInt (i : int) (j : int) = i < j" ;
-  "[@inline] let eqInt (i : int) (j : int) = i = j"
+  Definition address_ops :=
+    "[@inline] let eq_addr (a1 : address) (a2 : address) = a1 = a2".
+
+  Definition get_contract_def :=
+    <$
+    "let get_contract_unit (a : address) : unit contract  =" ;
+    "  match (Tezos.get_contract_opt a : unit contract option) with" ;
+    "    Some c -> c" ;
+    "  | None -> (failwith (""Contract not found."") : unit contract)"
+    $>.
+
+  Definition CameLIGO_call_ctx_type_name : string := "cctx".
+
+  Definition CameLIGO_call_ctx_type :=
+  <$ "(* ConCert's call context *)"
+  ; "type " ^ CameLIGO_call_ctx_type_name ^ " = {"
+  ; "  ctx_origin_ : address;"
+  ; "  ctx_from_ : address;"
+  ; "  ctx_contract_address_ : address;"
+  ; "  ctx_contract_balance_ : tez;"
+  ; "  ctx_amount_ : tez"
+  ; "}"
   $>.
 
-Definition tez_ops :=
-  <$
-  "[@inline] let addTez (n : tez) (m : tez) = n + m" ;
-  "[@inline] let subTez (n : tez) (m : tez) = n - m" ;
-  "[@inline] let leTez (a : tez ) (b : tez ) = a <= b" ;
-  "[@inline] let ltTez (a : tez ) (b : tez ) =  a < b" ;
-  "[@inline] let gtbTez (a : tez ) (b : tez ) =  a > b" ;
-  "[@inline] let eqTez (a : tez ) (b : tez ) = a = b" ;
-  "[@inline] let natural_to_mutez (a: nat): tez = a * 1mutez" ;
-  "[@inline] let divTez (a : tez) (b : tez) : tez = natural_to_mutez (a/b)" ;
-  "[@inline] let multTez (n : tez) (m : tez) = (n/1tez) * m";
-  "[@inline] let evenTez (i : tez) = (i mod 2n) = 0tez"
-  $>.
-Definition nat_ops :=
-  <$
-  "[@inline] let addN (a : nat ) (b : nat ) = a + b" ;
-  "[@inline] let multN (a : nat ) (b : nat ) = a * b" ;
-  "[@inline] let modN (a : nat ) (b : nat ) = a mod b" ;
-  "[@inline] let divN (a : nat ) (b : nat ) = a / b" ;
-  "[@inline] let eqN (a : nat ) (b : nat ) = a = b" ;
-  "[@inline] let lebN (a : nat ) (b : nat ) = a <= b" ;
-  "[@inline] let ltbN (a : nat ) (b : nat ) = a < b"
+  Definition CameLIGO_call_ctx_instance :=
+  <$"(* a call context instance with fields filled in with required data *)"
+  ; "let cctx_instance : " ^ CameLIGO_call_ctx_type_name ^ "= "
+  ; "{ ctx_origin_ = Tezos.source;"
+  ; "  ctx_from_ = Tezos.sender;"
+  ; "  ctx_contract_address_ = Tezos.self_address;"
+  ; "  ctx_contract_balance_ = Tezos.balance;"
+  ; "  ctx_amount_ = Tezos.balance"
+  ; "}"
+  ; ""
+  ; "(* context projections as functions *)"
+  ; "let ctx_from (c : " ^ CameLIGO_call_ctx_type_name ^ ") = c.ctx_from_"
+  ; "let ctx_origin (c : " ^ CameLIGO_call_ctx_type_name ^ ") = c.ctx_origin_"
+  ; "let ctx_contract_address (c : " ^ CameLIGO_call_ctx_type_name ^ ") = c.ctx_contract_address_"
+  ; "let ctx_contract_balance (c : " ^ CameLIGO_call_ctx_type_name ^ ") = c.ctx_contract_balance_"
+  ; "let ctx_amount (c : " ^ CameLIGO_call_ctx_type_name ^ ") = c.ctx_amount_"
   $>.
 
-Definition bool_ops :=
-  <$
-  "[@inline] let andb (a : bool ) (b : bool ) = a && b" ;
-  "[@inline] let orb (a : bool ) (b : bool ) = a || b"
+  Definition CameLIGO_chain_instance :=
+  <$ (* ConCert's Chain type and its instance. Currently we map all fields to Tezos.level *)
+  "type chain = {"
+  ; "  chain_height_     : nat;"
+  ; "  current_slot_     : nat;"
+  ; "  finalized_height_ : nat;"
+  ; "}"
+  ; ""
+  ; "let dummy_chain : chain = {"
+  ; "chain_height_     = Tezos.level;"
+  ; "current_slot_     = Tezos.level;"
+  ; "finalized_height_ = Tezos.level;"
+  ; "}"
+  ; ""
+  ; "(* chain projections as functions *)"
+  ; "let chain_height (c : chain ) = c.chain_height_"
+  ; "let current_slot (c : chain ) = c.current_slot_"
+  ; "let finalized_height (c : chain) = c.finalized_height_"
   $>.
 
-Definition time_ops :=
-  <$
-  "[@inline] let eqb_time (a1 : timestamp) (a2 : timestamp) = a1 = a2" ;
-  "[@inline] let leb_time (a1 : timestamp) (a2 : timestamp) = a1 <= a2" ;
-  "[@inline] let ltb_time (a1 : timestamp) (a2 : timestamp) = a1 < a2"
+  
+  Definition CameLIGO_Chain_CallContext :=
+  <$ CameLIGO_call_ctx_type
+   ; CameLIGO_call_ctx_instance
+   ; CameLIGO_chain_instance
   $>.
 
-Definition address_ops :=
-  "[@inline] let eq_addr (a1 : address) (a2 : address) = a1 = a2".
+  Definition CameLIGOPrelude :=
+    print_list id (nl ++ nl)
+               [int_ops; tez_ops; nat_ops;
+                bool_ops; time_ops; address_ops;
+                get_contract_def; CameLIGO_Chain_CallContext].
 
-Definition get_contract_def :=
-  <$
-  "let get_contract_unit (a : address) : unit contract  =" ;
-  "  match (Tezos.get_contract_opt a : unit contract option) with" ;
-  "    Some c -> c" ;
-  "  | None -> (failwith (""Contract not found."") : unit contract)"
-  $>.
+  Definition printWrapper (contract parameter_name storage_name : string): string :=
+    <$
+    "type return = (operation) list * (" ++ storage_name ++ " option)" ;
+    "type parameter_wrapper =" ;
+    "  Init of init_args_ty" ;
+    "| Call of " ++ parameter_name ++ " option" ;
+    "";
+    "let wrapper (param, st : parameter_wrapper * (" ++ storage_name ++ ") option) : return =" ;
+    "  match param with  " ;
+    "    Init init_args -> (([]: operation list), Some (init init_args))" ;
+    "  | Call p -> (" ;
+    "    match st with" ;
+    "      Some st -> (match (" ++ contract ++ " dummy_chain cctx_instance " ++ " st p) with   " ;
+    "                    Some v -> (v.0, Some v.1)" ;
+    "                  | None -> (failwith ("""") : return))" ;
+    "    | None -> (failwith (""cannot call this endpoint before Init has been called""): return))"
+    $>.
 
-Definition CameLIGO_call_ctx_type_name : string := "cctx".
+  Definition printMain (storage_name : string) :=
+    "let main (action, st : parameter_wrapper * " ++ storage_name ++ " option) : return = wrapper (action, st)".
 
-Definition CameLIGO_call_ctx_type :=
-<$ "(* ConCert's call context *)"
-; "type " ^ CameLIGO_call_ctx_type_name ^ " = {"
-; "  ctx_origin_ : address;"
-; "  ctx_from_ : address;"
-; "  ctx_contract_address_ : address;"
-; "  ctx_contract_balance_ : tez;"
-; "  ctx_amount_ : tez"
-; "}"
-$>.
+    Definition print_default_entry_point (state_nm : kername) (receive_nm : kername) (msg_nm : kername) :=
+  let st := print_type_name state_nm in
+  let rec := print_const_name receive_nm in
+  let msg := print_type_name msg_nm in
+  <$ printWrapper rec msg st;
+     "";
+     printMain st $>.
 
-Definition CameLIGO_call_ctx_instance :=
-<$"(* a call context instance with fields filled in with required data *)"
-; "let cctx_instance : " ^ CameLIGO_call_ctx_type_name ^ "= "
-; "{ ctx_origin_ = Tezos.source;"
-; "  ctx_from_ = Tezos.sender;"
-; "  ctx_contract_address_ = Tezos.self_address;"
-; "  ctx_contract_balance_ = Tezos.balance;"
-; "  ctx_amount_ = Tezos.balance"
-; "}"
-; ""
-; "(* projections as functions *)"
-; "let ctx_from (c : " ^ CameLIGO_call_ctx_type_name ^ ") = c.ctx_from_"
-; "let ctx_contract_address (c : " ^ CameLIGO_call_ctx_type_name ^ ") = c.ctx_contract_address_"
-; "let ctx_contract_balance (c : " ^ CameLIGO_call_ctx_type_name ^ ") = c.ctx_contract_balance_"
-; "let ctx_amount_ (c : " ^ CameLIGO_call_ctx_type_name ^ ") = c.ctx_amount_"
-$>.
-
-Definition dummy_chain :=
-<$ (* ConCert's Chain type and its isntance. Currently we map all fields to Tezos.level *)
-"type chain = {"
-; "  chain_height     : nat;"
-; "  current_slot     : nat;"
-; "  finalized_height : nat;"
-; "}"
-; ""
-; "let dummy_chain : chain = {"
-; "chain_height     = Tezos.level;"
-; "current_slot     = Tezos.level;"
-; "finalized_height = Tezos.level;"
-; "}"
-$>.
-
-Definition CameLIGO_Chain_CallContext :=
-<$ CameLIGO_call_ctx_type
-; CameLIGO_call_ctx_instance
-; dummy_chain
-$>.
-
-Definition CameLIGOPrelude :=
-  print_list id (nl ++ nl)
-             [int_ops; tez_ops; nat_ops;
-              bool_ops; time_ops; address_ops;
-              get_contract_def; CameLIGO_Chain_CallContext].
-
-Definition printWrapper (contract parameter_name storage_name : string): string :=
-  <$
-  "type return = (operation) list * (" ++ storage_name ++ " option)" ;
-  "type parameter_wrapper =" ;
-  "  Init of init_args_ty" ;
-  "| Call of " ++ parameter_name ++ " option" ;
-  "";
-  "let wrapper (param, st : parameter_wrapper * (" ++ storage_name ++ ") option) : return =" ;
-  "  match param with  " ;
-  "    Init init_args -> (([]: operation list), Some (init init_args))" ;
-  "  | Call p -> (" ;
-  "    match st with" ;
-  "      Some st -> (match (" ++ contract ++ " dummy_chain cctx_instance " ++ " st p) with   " ;
-  "                    Some v -> (v.0, Some v.1)" ;
-  "                  | None -> (failwith ("""") : return))" ;
-  "    | None -> (failwith (""cannot call this endpoint before Init has been called""): return))"
-  $>.
-
-Definition printMain (storage_name : string) :=
-  "let main (action, st : parameter_wrapper * " ++ storage_name ++ " option) : return = wrapper (action, st)".
+End PPLigo.
