extraction/examples/CameLIGOExtractionTests.v
@@ -30,7 +30,8 @@ Local Open Scope string_scope.
 Import MonadNotation.
 Open Scope Z.
 
-Definition PREFIX := "".
+Existing Instance PrintConfShortNames.PrintWithShortNames.
+
 Definition bindOptCont {A B} (a : option A) (f : A -> option B) : option B :=
   match a with
   | Some a => f a
@@ -77,7 +78,6 @@ Module SafeHead.
 
     Time MetaCoq Run
          (t <- CameLIGO_extract_single
-                PREFIX
                 safe_head_inline
                 TT_consts TT_ctors
                 ""
@@ -144,7 +144,6 @@ Module Counter.
 
         (* and a test address *)
         lmd_prelude := CameLIGOPrelude ++ nl
-                       ++ dummy_chain ++ nl
                        ++ "let test_account : address = (""tz1KqTpEZ7Yob7QbPE4Hy4Wo8fHG8LhKxZSx"" : address)";
 
         (* initial storage *)
@@ -160,7 +159,7 @@ Module Counter.
 
         (* code for the entry point *)
         lmd_entry_point :=
-          CameLIGOPretty.printWrapper (PREFIX ++ "counter") "msg" "storage" ++ nl
+          CameLIGOPretty.printWrapper ("counter") "msg" "storage" ++ nl
           ++ CameLIGOPretty.printMain "storage" |}.
 
 End Counter.
@@ -179,10 +178,10 @@ Section CounterExtraction.
       It uses the certified erasure from [MetaCoq] and the certified deboxing procedure
       that removes application of boxes to constants and constructors. *)
 
-  (* NOTE: running computations inside [TemplateMonad] is quite slow. That's why we comment out this code and use a different way below *)
+  (** NOTE: running computations inside [TemplateMonad] is quite slow. That's why we comment out this code and use a different way below *)
 
   (* Time MetaCoq Run *)
-  (*     (t <- CameLIGO_extract PREFIX [] TT_remap_counter [] CameLIGO_call_ctx LIGO_COUNTER_MODULE ;; *)
+  (*     (t <- CameLIGO_extract [] TT_remap_counter [] CameLIGO_call_ctx LIGO_COUNTER_MODULE ;; *)
   (*       tmDefinition LIGO_COUNTER_MODULE.(lmd_module_name) t). *)
 
 
@@ -192,7 +191,7 @@ Section CounterExtraction.
   (** This command adds [cameLIGO_counter_prepared] to the environment,
       which can be evaluated later *)
   Time MetaCoq Run
-       (CameLIGO_prepare_extraction PREFIX [] TT_remap_counter [] "cctx_instance" LIGO_COUNTER_MODULE).
+       (CameLIGO_prepare_extraction [] TT_remap_counter TT_rename_ctors_default "cctx_instance" LIGO_COUNTER_MODULE).
 
   Time Definition cameLIGO_counter_1 := Eval vm_compute in cameLIGO_counter_prepared.
 
@@ -255,8 +254,6 @@ Defined.
       lmd_prelude :=
         CameLIGOPrelude
           ++ nl
-          ++ dummy_chain
-          ++ nl
           ++ nl
           ++ "let test_account : address = (""tz1KqTpEZ7Yob7QbPE4Hy4Wo8fHG8LhKxZSx"" : address)"
           ++ nl
@@ -276,7 +273,7 @@ Defined.
 
       (* code for the entry point *)
       lmd_entry_point :=
-        "type storage = ((time_coq * (tez * address)) * ((address,tez) map * bool))" ++ CameLIGOPretty.printWrapper (PREFIX ++ "crowdfunding_receive")
+        "type storage = ((time_coq * (tez * address)) * ((address,tez) map * bool))" ++ CameLIGOPretty.printWrapper ("crowdfunding_receive")
                                     "msg_coq"
                                     "storage"
                                     ++ nl
@@ -313,14 +310,8 @@ Section CrowdfundingExtraction.
   ; remap <%% lookup_map' %%> "Map.find_opt"
   ].
 
-  Definition TT_rename_crowdfunding :=
-    [ ("mnil", "(Map.empty : (address,tez) map)")
-    ; ("true", "true")
-    ; ("false", "false")
-    ; ("tt", "()")].
-
   Time MetaCoq Run
-       (CameLIGO_prepare_extraction PREFIX [] TT_remap_crowdfunding TT_rename_crowdfunding "cctx_instance" CF_MODULE).
+       (CameLIGO_prepare_extraction [] TT_remap_crowdfunding TT_rename_ctors_default "cctx_instance" CF_MODULE).
 
   Time Definition cameLIGO_crowdfunding := Eval vm_compute in cameLIGO_crowdfunding_prepared.
 
@@ -411,17 +402,17 @@ Section EIP20TokenExtraction.
     ].
 
 
-  Definition TT_rename_eip20token :=
-    [ ("Z0" ,"0tez")
-    ; ("N0", "0")
-    ; ("N1", "1")
-    ; ("nil", "[]")
-    ; ("true", "true")
-    ; ("false", "false")
-    ; ("tt", "()") ].
+  (* Definition TT_rename_eip20token := *)
+  (*   [ ("Z0" ,"0tez") *)
+  (*   ; ("N0", "0") *)
+  (*   ; ("N1", "1") *)
+  (*   ; ("nil", "[]") *)
+  (*   ; ("true", "true") *)
+  (*   ; ("false", "false") *)
+  (*   ; ("tt", "()") ]. *)
 
   Time MetaCoq Run
-  (CameLIGO_prepare_extraction PREFIX TT_inlines_eip20token TT_remap_eip20token TT_rename_eip20token "cctx_instance" LIGO_EIP20Token_MODULE).
+  (CameLIGO_prepare_extraction TT_inlines_eip20token TT_remap_eip20token TT_rename_ctors_default "cctx_instance" LIGO_EIP20Token_MODULE).
 
   Time Definition cameLIGO_eip20token := Eval vm_compute in cameLIGO_eip20token_prepared.
 
