extraction/examples/Dexter2Extract.v
@@ -1,0 +1,212 @@
+(** * Extraction of Dexter 2 to CameLIGO *)
+
+From Coq Require Import PeanoNat ZArith Notations.
+From Coq Require Import List Ascii String Bool.
+
+From MetaCoq.Template Require Import All.
+
+From ConCert.Embedding Require Import Notations.
+From ConCert.Embedding Require Import MyEnv CustomTactics.
+From ConCert.Embedding Require Import Notations.
+From ConCert.Extraction Require Import Common Optimize.
+From ConCert.Extraction Require Import CameLIGOPretty CameLIGOExtract.
+From ConCert.Execution Require Import Serializable.
+From ConCert.Execution Require Import Blockchain.
+From ConCert.Execution.Examples Require Dexter2CPMM.
+From ConCert.Execution Require Import Containers.
+From ConCert.Utils Require Import RecordUpdate.
+From ConCert.Utils Require Import StringExtra.
+
+From stdpp Require gmap.
+
+
+Local Open Scope string_scope.
+
+Import MonadNotation.
+Open Scope Z.
+
+(** Exposing a printing configuration *)
+Existing Instance PrintConfAddModuleNames.PrintWithModuleNames.
+
+Section Dexter2Extraction.
+
+  Context `{ChainBase}.
+
+  Import Dexter2CPMM.
+  Import RecordSetNotations.
+
+  Open Scope Z_scope.
+
+  Definition init (ctx : ContractCallContext) (setup : Setup) : option State :=
+    let ctx_ := ctx in
+    Some {|
+        tokenPool := 0;
+        xtzPool := 0;
+        lqtTotal := setup.(lqtTotal_);
+        selfIsUpdatingTokenPool := false;
+        freezeBaker := false;
+        manager := setup.(manager_);
+        tokenAddress := setup.(tokenAddress_);
+        tokenId := setup.(tokenId_);
+        lqtAddress := null_address
+      |}.
+
+  Definition receive_ (chain : Chain)
+       (ctx : ContractCallContext)
+       (state : State)
+       (maybe_msg : option Msg)
+    : option (list ActionBody * State) :=
+    match receive chain ctx state maybe_msg with
+    | Some x => Some (x.2, x.1)
+    | None => None
+    end.
+  Close Scope Z_scope.
+
+  Definition call_to_token_ligo : string :=
+    <$ "let call_to_token (addr : address) (amt : nat) (msg : _msg) : operation =" ;
+       "  let token_ : _msg contract =";
+       "  match (Tezos.get_contract_opt (addr) : _msg contract option) with";
+       "    Some contract -> contract";
+       "  | None -> (failwith ""Contract not found."" : _msg contract) in";
+       "  Tezos.transaction msg (natural_to_mutez amt) token_" $>.
+
+  (** Next two definition are borrowed from the actual Dexter 2 implementation
+       https://gitlab.com/dexter2tz/dexter2tz/-/blob/master/dexter.mligo *)
+  Definition natural_to_mutez_ligo : string :=
+    "[@inline] let natural_to_mutez (a: nat): tez = a * 1mutez".
+
+  Definition mutez_to_natural_ligo : string :=
+    "[@inline] let mutez_to_natural (a: tez): nat = a / 1mutez".
+
+  (** We change the signature of the original definition slightly, so it takes a [nat] and converts
+      in to [tez]. We also return [operation option] instead of failing *)
+  Definition xtz_transfer_ligo : string :=
+    <$ "let xtz_transfer (to_ : address) (amount_ : nat) : operation option =";
+       "  match (Tezos.get_contract_opt to_ : unit contract option) with";
+       "    | None -> None";
+       "    | Some c -> Some (Tezos.transaction () (natural_to_mutez amount_) c)" $>.
+
+  Definition subNatTruncated_ligo : string :=
+    "let subNTruncated (n : nat) (m : nat) : nat = if n < m then 0n else abs (n-m)".
+
+  Definition LIGO_DEXTER2_MODULE : CameLIGOMod Msg ContractCallContext Setup State ActionBody :=
+  {| (* a name for the definition with the extracted code *)
+     lmd_module_name := "cameLIGO_dexter2" ;
+
+      (* definitions of operations on pairs and ints *)
+     lmd_prelude := CameLIGOPrelude ++ nl ++ nl ++
+                    <$ call_to_token_ligo;
+                       "";
+                       natural_to_mutez_ligo;
+                       "";
+                       mutez_to_natural_ligo;
+                       "";
+                       xtz_transfer_ligo;
+                       "";
+                       subNatTruncated_ligo $>;
+
+      (* initial storage *)
+      lmd_init := init ;
+
+      (* NOTE: printed as local [let]-bound definitions in the init *)
+      lmd_init_prelude := "";
+
+      (* TODO: maybe not needed, [lmd_prelude] should be enough *)
+      lmd_receive_prelude := "";
+
+      (* the main functionality *)
+      lmd_receive := receive_ ;
+
+      (* code for the entry point *)
+    lmd_entry_point := print_default_entry_point <%% @State %%>
+                                                 <%% @receive_ %%>
+                                                 <%% @Msg %%> |}.
+
+  Definition TT_remap_arith : list (kername * string) :=
+[   remap <%% Z %%> "int"
+  ; remap <%% N %%> "nat"
+  ; remap <%% nat %%> "nat"
+
+  ; remap <%% Nat.add %%> "addN"
+  ; remap <%% Nat.leb %%> "lebN"
+  ; remap <%% Nat.ltb %%> "ltbN"
+  ; remap <%% Nat.mul %%> "multN"
+
+  ; remap <%% Pos.add %%> "addN"
+  ; remap <%% Pos.sub %%> "subN"
+  ; remap <%% Pos.mul %%> "multN"
+  ; remap <%% Pos.leb %%> "leN"
+  ; remap <%% Pos.eqb %%> "eqN"
+  ; remap <%% Z.add %%> "addInt"
+  ; remap <%% Z.sub %%> "subInt"
+  ; remap <%% Z.mul %%> "multInt"
+  ; remap <%% Z.div %%> "divInt"
+  ; remap <%% Z.leb %%> "leInt"
+  ; remap <%% Z.ltb %%> "ltInt"
+  ; remap <%% Z.eqb %%> "eqInt"
+  ; remap <%% Z.gtb %%> "gtbInt"
+  ; remap <%% Z.even %%> "evenInt"
+  ; remap <%% N.add %%> "addN"
+  ; remap <%% N.sub %%> "subNTruncated"
+  ; remap <%% N.mul %%> "multN"
+  ; remap <%% N.leb %%> "lebN"
+  ; remap <%% N.ltb %%> "ltbN"
+  ; remap <%% N.eqb %%> "eqN"
+  ; remap <%% Dexter2CPMM.div %%> "divN_opt"
+  ; remap <%% N.modulo %%> "moduloN"
+  ; remap <%% N.sub %%> "subOption"
+  ; remap <%% Z.to_N %%> "mutez_to_natural"
+  ; remap <%% Z.of_N %%> "z_of_N"
+  ; remap <%% non_zero_amount %%> "(fun (x : tez) -> 0tez < x)"
+].
+
+  Definition TT_remap_dexter2 : list (kername * string) :=
+   [
+    remap <%% @ContractCallContext %%> CameLIGO_call_ctx_type_name
+  ; remap <%% @FMap %%> "map"
+  ; remap <%% @Common.AddressMap.add %%> "Map.add"
+  ; remap <%% @Common.AddressMap.find %%> "Map.find_opt"
+  ; remap <%% @Common.AddressMap.empty %%> "Map.empty"
+  ; remap <%% @FMap.add %%> "Map.add"
+  ; remap <%% @FMap.find %%> "Map.find_opt"
+  ; remap <%% @FMap.empty %%> "Map.empty"
+
+  ; remap <%% @call_to_token %%> "call_to_token"
+  ; remap <%% @call_to_other_token %%> "call_to_token"
+  ; remap <%% @xtz_transfer %%> "xtz_transfer"
+  ; remap <%% @call_liquidity_token %%> "call_to_token"
+  ; remap <%% token_id %%> "nat"
+
+  ; remap <%% @null_address %%> "(""tz1Ke2h7sDdakHJQh8WX4Z372du1KChsksyU"" : address)"
+  ; remap <%% @Serializable %%> "" (* FIXME: workaround; should be ignored instead *)
+  ; remap <%% @DexterMsg_serializable %%> "" (* FIXME: workaround; should be ignored instead *)
+   ].
+
+  Definition TT_remap_all :=
+    (TT_remap_arith ++ TT_remap_dexter2)%list.
+
+  Definition TT_inlines_dexter2 : list kername :=
+    [
+      <%% Monads.Monad_option %%>
+    ; <%% @Monads.bind %%>
+    ; <%% @Monads.ret %%>
+    ; <%% @Extras.with_default %%>
+
+    ; <%% @SetterFromGetter %%> ].
+
+  Time MetaCoq Run
+  (CameLIGO_prepare_extraction TT_inlines_dexter2 TT_remap_all TT_rename_ctors_default "cctx_instance" LIGO_DEXTER2_MODULE).
+
+  (* Time MetaCoq Run *)
+  (* (CameLIGO_prepare_extraction [] TT_remap_dexter2 TT_rename_dexter2 "cctx_instance" LIGO_DEXTER2_MODULE). *)
+
+
+  Time Definition cameLIGO_dexter2 := Eval vm_compute in cameLIGO_dexter2_prepared.
+
+  MetaCoq Run (tmMsg cameLIGO_dexter2).
+
+  (** We redirect the extraction result for later processing and compiling with the CameLIGO compiler *)
+  (* Redirect "examples/extracted-code/cameligo-extract/dexter2CertifiedExtraction.mligo" *)
+  (* MetaCoq Run (tmMsg cameLIGO_dexter2). *)
+
+End Dexter2Extraction.
